theories/Ownership.v
@@ -1,0 +1,24 @@
+From LinearCore Require
+  Reflect
+  .
+
+
+
+Variant ownership : Set :=
+  | Owned
+  | Referenced
+  .
+
+Definition eq a b :=
+  match a, b with
+  | Owned, Owned
+  | Referenced, Referenced => true
+  | _, _ => false
+  end.
+
+Lemma eq_spec a b
+  : Reflect.Bool (a = b) (eq a b).
+Proof. destruct a; destruct b; constructor; try reflexivity; intro D; discriminate D. Qed.
+
+Definition owned ownership := match ownership with Owned => true | Referenced => false end.
+Arguments owned ownership/.
